CorrectnessProof.v
@@ -1,0 +1,67 @@
+Require Import Derivation.
+Require Import Grammar.
+Require Import List.
+Require Import Parser.
+Require Import String.
+Import ListNotations.
+Open Scope string_scope.
+
+Ltac inv H := inversion H; clear H; subst.
+
+Theorem epsilon_preserves_truth :
+  forall (pt : M.t (M.t (list production)))
+         (stack' : list symbol)
+         (tokens : list string)
+         (fuel : nat),
+    parseLoop pt (EPS :: stack') tokens (S fuel) = true ->
+    parseLoop pt stack' tokens fuel = true.
+Proof.
+  intros. inv H. reflexivity.
+Defined.
+
+Theorem terminal_match_preserves_truth :
+  forall (pt : M.t (M.t (list production)))
+         (tName : string)
+         (stack' : list symbol)
+         (token : string)
+         (tokens : list string)
+         (fuel : nat),
+    parseLoop pt (T tName :: stack') (token :: tokens)
+              (S fuel) = true ->
+    parseLoop pt stack' tokens fuel = true.
+Proof.
+  intros. inv H. destruct (cmpSymbol (T tName) (T token)).
+  - reflexivity.
+  - inv H1.
+Defined.
+
+Theorem nonterminal_expansion_preserves_truth : 
+  forall (pt : M.t (M.t (list production)))
+         (ntName : string)
+         (stack' : list symbol)
+         (ys : list symbol)
+         (token : string)
+         (tokens : list string)
+         (fuel : nat),
+    parseLoop pt (NT ntName :: stack') (token :: tokens)
+              (S fuel) = true ->
+    exists (x : symbol) (ys : list symbol),
+      ptLookup (NT ntName) (T token) pt = Some (x, ys) /\
+      parseLoop pt (ys ++ stack') (token :: tokens) fuel = true.
+Proof.
+  intros. inv H.
+  destruct (ptLookup (NT ntName) (T token)).
+  - destruct p. exists s. exists l. split; reflexivity.
+  - inversion H1.
+Defined.
+
+    
+Theorem parse'_correct : forall (prefix : list string) (fuel : nat),
+    parse' (mkParseTable g311 100) (NT "S") prefix fuel = true ->
+    exists (pt : ast), @derives g311 (NT "S") prefix pt.
+Proof. intros. induction fuel.
+       - inversion H.
+       - destruct prefix.
+         + inversion H.
+
+
