Grammar.v
@@ -3,6 +3,10 @@ Require Import Parser.
 Require Import String.
 Import ListNotations.
 
+Definition gSimple : grammar :=
+  [(NT "A", [T "a"; T "b"]);
+   (NT "X", [T "x"; T "y"])].
+
 Definition g311 : grammar :=
   [(NT "S", [T "if" ; NT "E" ; T "then" ; NT "S" ; T "else" ; NT "S"]) ;
    (NT "S", [T "begin" ; NT "S" ; NT "L"]) ;
