compile.sh
@@ -1,0 +1,14 @@
+#!/bin/bash
+
+
+SOURCE_FILES=("Parser.v"
+	      "Grammar.v"
+	      "Derivation.v"
+	      "ParserTest.v"
+	      "DerivationTest.v"
+	     )
+
+
+for v_file in "${SOURCE_FILES[@]}"; do
+    coqc "${v_file}"
+done
